hard case of OneLeaderLogPerTerm

raft-proofs/OneLeaderLogPerTermProof.v
@@ -4,27 +4,372 @@ Import ListNotations.
 Require Import VerdiTactics.
 Require Import Util.
 Require Import Net.
+Require Import Omega.
 
 Require Import Raft.
 Require Import RaftRefinementInterface.
 Require Import CommonDefinitions.
+Require Import CommonTheorems.
+Require Import SpecLemmas.
+Require Import RefinementSpecLemmas.
+Require Import RefinementCommonTheorems.
 
+Require Import UpdateLemmas.
+Local Arguments update {_} {_} {_} _ _ _ _ : simpl never.
+
+Require Import LeaderLogsVotesWithLogInterface.
+Require Import VotesCorrectInterface.
+Require Import CroniesCorrectInterface.
+Require Import VotesVotesWithLogCorrespondInterface.
 Require Import OneLeaderLogPerTermInterface.
 
 Section OneLeaderLogPerTerm.
   Context {orig_base_params : BaseParams}.
   Context {one_node_params : OneNodeParams orig_base_params}.
   Context {raft_params : RaftParams orig_base_params}.
+  Context {rri : raft_refinement_interface}.
 
-  Theorem one_leaderLog_per_term_invariant :
+  Context {llvwli : leaderLogs_votesWithLog_interface}.
+  Context {vci : votes_correct_interface}.
+  Context {cci : cronies_correct_interface}.
+  Context {vvci : votes_votesWithLog_correspond_interface}.
+
+  Ltac update_destruct :=
+    match goal with
+      | [ |- context [ update _ ?y _ ?x ] ] => destruct (name_eq_dec y x)
+      | [ H : context [ update _ ?y _ ?x ] |- _ ] => destruct (name_eq_dec y x)
+    end.
+
+  Ltac start :=
+    red; unfold one_leaderLog_per_term; simpl; intros.
+
+  Ltac start_update :=
+    start;
+    repeat find_higher_order_rewrite;
+    repeat (update_destruct; subst; rewrite_update);
+    [| | |eauto].
+
+  (*Lemma one_leaderLog_per_term_unchanged :
+    forall net st' h gd d ps',
+      one_leaderLog_per_term net ->
+      (forall h' : Net.name, st' h' = update (nwState net) h (gd, d) h') ->
+      leaderLogs gd = leaderLogs (fst (nwState net h)) ->
+      currentTerm d >= currentTerm (snd (nwState net h)) ->
+      one_leaderLog_per_term {| nwPackets := ps'; nwState := st' |}.
+  Proof.
+    unfold one_leaderLog_per_term. intros. find_higher_order_rewrite.
+    update_destruct; subst; rewrite_update.
+    - simpl in *. find_rewrite. find_apply_hyp_hyp. omega.
+    - eauto.
+  Qed.
+
+  Ltac currentTerm_sanity_unchanged :=
+    red; intros; eapply one_leaderLog_per_term_unchanged; subst; eauto.
+
+  Ltac currentTerm_sanity_break_update :=
+    currentTerm_sanity_start_update;
+    match goal with
+      h : _ |- _ => eapply h
+    end; [| eauto];
+    match goal with
+      h : _ |- _ => solve [rewrite h; auto]
+    end.*)
+
+  Lemma one_leaderLog_per_term_init :
+    refined_raft_net_invariant_init one_leaderLog_per_term.
+  Proof.
+    start. contradiction.
+  Qed.
+
+  Lemma one_leaderLog_per_term_client_request :
+    refined_raft_net_invariant_client_request one_leaderLog_per_term.
+  Proof.
+    start_update; simpl in *.
+    - repeat find_rewrite_lem update_elections_data_client_request_leaderLogs. eauto.
+    - repeat find_rewrite_lem update_elections_data_client_request_leaderLogs. eauto.
+    - repeat find_rewrite_lem update_elections_data_client_request_leaderLogs. eauto.
+  Qed.
+
+  Lemma one_leaderLog_per_term_timeout :
+    refined_raft_net_invariant_timeout one_leaderLog_per_term.
+  Proof.
+    admit.
+    (*currentTerm_sanity_unchanged.
+    - apply update_elections_data_timeout_leaderLogs.
+    - find_apply_lem_hyp handleTimeout_type_strong. intuition.*)
+  Qed.
+
+  Lemma one_leaderLog_per_term_append_entries :
+    refined_raft_net_invariant_append_entries one_leaderLog_per_term.
+  Proof.
+    admit.
+    (*currentTerm_sanity_unchanged.
+    - apply update_elections_data_appendEntries_leaderLogs.
+    - find_apply_lem_hyp handleAppendEntries_type_term. intuition.*)
+  Qed.
+
+  Lemma one_leaderLog_per_term_append_entries_reply :
+    refined_raft_net_invariant_append_entries_reply one_leaderLog_per_term.
+  Proof.
+    admit.
+    (*currentTerm_sanity_unchanged.
+    - find_apply_lem_hyp handleAppendEntriesReply_type_term. intuition.*)
+  Qed.
+
+  Lemma one_leaderLog_per_term_request_vote :
+    refined_raft_net_invariant_request_vote one_leaderLog_per_term.
+  Proof.
+    admit.
+    (*currentTerm_sanity_unchanged.
+    - apply leaderLogs_update_elections_data_requestVote.
+    - find_apply_lem_hyp handleRequestVote_type_term. intuition.*)
+  Qed.
+
+  Definition leaderLogs_currentTerm_sanity_candidate (net : network) : Prop :=
+    forall h t log,
+      type (snd (nwState net h)) = Candidate ->
+      In (t, log) (leaderLogs (fst (nwState net h))) ->
+      t < currentTerm (snd (nwState net h)).
+
+  Theorem leaderLogs_currentTerm_sanity_candidate_invariant :
+    forall net,
+      refined_raft_intermediate_reachable net ->
+      leaderLogs_currentTerm_sanity_candidate net.
+  Admitted.
+
+  Lemma update_elections_data_requestVoteReply_leaderLogs' :
+    forall h h' t st t' ll' r,
+      In (t', ll') (leaderLogs (update_elections_data_requestVoteReply h h' t r st)) ->
+      In (t', ll') (leaderLogs (fst st))
+      \/ (r = true
+          /\ t = currentTerm (snd st)
+          /\ ll' = log (snd st)
+          /\ t' = currentTerm (snd st)
+          /\ type (snd st) = Candidate
+          /\ wonElection (dedup name_eq_dec (h' :: votesReceived (snd st))) = true).
+  Proof.
+    unfold update_elections_data_requestVoteReply.
+    intros.
+    repeat break_match; auto.
+    simpl in *. intuition.
+    find_inversion. right.
+    unfold handleRequestVoteReply in *.
+    repeat break_match; simpl in *; intuition; try congruence;
+    break_if; try congruence; do_bool; eauto using le_antisym.
+  Qed.
+
+  Ltac unfold_invariant hyp :=
+    (red in hyp;  (* try unfolding the invariant and look for conjunction *)
+      match type of hyp with
+        | _ /\ _ => break_and
+        | _ => fail 1  (* better to not unfold *)
+      end) ||
+    break_and.
+
+  (* introduces a refined invariant then tries to break apart any nested
+     conjunctions to return the usable invariants as hypotheses *)
+  Ltac intro_invariant lem :=
+    match goal with
+    | [ h: refined_raft_intermediate_reachable _ |- _ ] =>
+        let x := fresh in
+        pose proof h as x;
+          apply lem in x;
+          unfold_invariant x
+    end.
+
+  Lemma wonElection_length :
+    forall votes,
+      wonElection votes = true ->
+      length votes > div2 (length nodes).
+  Proof.
+    unfold wonElection. intros. find_apply_lem_hyp leb_true_le. omega.
+  Qed.
+
+  Lemma pigeon_nodes :
+    forall (q1 q2 : list name),
+      NoDup q1 ->
+      NoDup q2 ->
+      length q1 > div2 (length nodes) ->
+      length q2 > div2 (length nodes) ->
+      exists v, In v q1 /\ In v q2.
+  Proof.
+    intros. eapply pigeon with (l := nodes).
+    - apply name_eq_dec.
+    - intros. apply (@all_names_nodes _ multi_params).
+    - intros. apply (@all_names_nodes _ multi_params).
+    - apply (@no_dup_nodes _ multi_params).
+    - assumption.
+    - assumption.
+    - apply div2_correct; assumption.
+  Qed.
+
+  (* two different hosts cannot both have the same term in their leader logs *)
+  (*Lemma contradiction_case :
+    forall (net : network (params := refined_multi_params)) t ll ll' (h h' : name) (p : packet (params := refined_multi_params)) t0 v xs ys,
+      refined_raft_intermediate_reachable net ->
+      pBody p = RequestVoteReply t v ->
+      nwPackets net = xs ++ p :: ys ->
+      In (t, ll) (leaderLogs (fst (nwState net h))) ->
+      In (t, ll') (leaderLogs (update_elections_data_requestVoteReply (pDst p) (pSrc p) t0 v (nwState net (pDst p)))) ->
+      pDst p = h' ->
+      pDst p <> h ->
+      False.
+  Proof.
+    intros. unfold not in *. find_false.
+    simpl in *. find_apply_lem_hyp update_elections_data_requestVoteReply_leaderLogs'.
+    intro_invariant leaderLogs_votesWithLog_invariant.
+    break_or_hyp; repeat (apply_prop_hyp leaderLogs_votesWithLog In; break_exists).
+    - assert (exists h, In h x /\ In h x0) by (apply pigeon_nodes; intuition).
+      break_exists; break_and.
+      do 2 (find_apply_hyp_hyp; break_exists; break_and).
+      intro_invariant votes_votesWithLog_correspond_invariant.
+      do 2 (apply_prop_hyp votes_votesWithLog In).
+      intro_invariant votes_correct_invariant.
+      eauto.
+    - assert (exists h, In h x /\ In h (dedup name_eq_dec (pSrc p :: votesReceived (snd (nwState net (pDst p)))))).
+      { eapply pigeon_nodes.
+        - intuition.
+        - apply NoDup_dedup.
+        - intuition.
+        - apply wonElection_length; intuition. }
+      break_exists. break_and.
+      find_apply_hyp_hyp; break_exists; break_and.
+      intro_invariant votes_votesWithLog_correspond_invariant.
+      apply_prop_hyp votes_votesWithLog In.
+      find_apply_lem_hyp in_dedup_was_in.
+      simpl in *.
+      intro_invariant cronies_correct_invariant.
+      intro_invariant votes_correct_invariant.
+      break_or_hyp; eauto.
+  Qed.*)
+
+  Lemma one_leaderLog_per_term_request_vote_reply :
+    refined_raft_net_invariant_request_vote_reply one_leaderLog_per_term.
+  Proof.
+    start. repeat find_higher_order_rewrite. repeat (update_destruct; rewrite_update).
+    - split; [subst; auto|].
+      find_copy_eapply_lem_hyp leaderLogs_update_elections_data_RVR; [|eauto].
+      pose proof H.
+      eapply leaderLogs_update_elections_data_RVR with (ll0 := ll) in H; [|eauto].
+      intro_invariant leaderLogs_currentTerm_sanity_candidate_invariant.
+      intuition.
+      + match goal with
+        | [ h: _ |- _ ] => solve[eapply h; eauto]
+        end.
+      + apply_prop_hyp leaderLogs_currentTerm_sanity_candidate nwState; auto.
+        find_copy_apply_lem_hyp handleRequestVoteReply_type. intuition; unfold raft_data in *; simpl in *.
+        * subst. repeat find_rewrite. discriminate.
+        * find_apply_lem_hyp lt_asym. congruence.
+        * subst. repeat find_rewrite. find_apply_lem_hyp lt_irrefl. contradiction.
+      + apply_prop_hyp leaderLogs_currentTerm_sanity_candidate nwState; auto.
+        find_copy_apply_lem_hyp handleRequestVoteReply_type. intuition; unfold raft_data in *; simpl in *.
+        * subst. repeat find_rewrite. discriminate.
+        * find_apply_lem_hyp lt_asym. congruence.
+        * subst. repeat find_rewrite. find_apply_lem_hyp lt_irrefl. contradiction.
+      + subst. auto.
+    - intros. unfold not in *. find_false.
+      simpl in *. find_apply_lem_hyp update_elections_data_requestVoteReply_leaderLogs'.
+      intro_invariant leaderLogs_votesWithLog_invariant.
+      break_or_hyp; repeat (apply_prop_hyp leaderLogs_votesWithLog In; break_exists).
+      + assert (exists h, In h x /\ In h x0) by (apply pigeon_nodes; intuition).
+        break_exists; break_and.
+        do 2 (find_apply_hyp_hyp; break_exists; break_and).
+        intro_invariant votes_votesWithLog_correspond_invariant.
+        do 2 (apply_prop_hyp votes_votesWithLog In).
+        intro_invariant votes_correct_invariant.
+        eauto.
+      + assert (exists h, In h x /\ In h (dedup name_eq_dec (pSrc p :: votesReceived (snd (nwState net (pDst p)))))).
+        { eapply pigeon_nodes.
+          - intuition.
+          - apply NoDup_dedup.
+          - intuition.
+          - apply wonElection_length; intuition. }
+        break_exists. break_and.
+        find_apply_hyp_hyp; break_exists; break_and.
+        intro_invariant votes_votesWithLog_correspond_invariant.
+        apply_prop_hyp votes_votesWithLog In.
+        find_apply_lem_hyp in_dedup_was_in.
+        simpl in *.
+        intro_invariant cronies_correct_invariant.
+        intro_invariant votes_correct_invariant.
+        break_or_hyp; eauto.
+    - intros. unfold not in *. find_false.
+      simpl in *. find_apply_lem_hyp update_elections_data_requestVoteReply_leaderLogs'.
+      intro_invariant leaderLogs_votesWithLog_invariant.
+      break_or_hyp; repeat (apply_prop_hyp leaderLogs_votesWithLog In; break_exists).
+      + assert (exists h, In h x /\ In h x0) by (apply pigeon_nodes; intuition).
+        break_exists; break_and.
+        do 2 (find_apply_hyp_hyp; break_exists; break_and).
+        intro_invariant votes_votesWithLog_correspond_invariant.
+        do 2 (apply_prop_hyp votes_votesWithLog In).
+        intro_invariant votes_correct_invariant.
+        eauto.
+      + assert (exists h, In h x /\ In h (dedup name_eq_dec (pSrc p :: votesReceived (snd (nwState net (pDst p)))))).
+        { eapply pigeon_nodes.
+          - intuition.
+          - apply NoDup_dedup.
+          - intuition.
+          - apply wonElection_length; intuition. }
+        break_exists. break_and.
+        find_apply_hyp_hyp; break_exists; break_and.
+        intro_invariant votes_votesWithLog_correspond_invariant.
+        apply_prop_hyp votes_votesWithLog In.
+        find_apply_lem_hyp in_dedup_was_in.
+        simpl in *.
+        intro_invariant cronies_correct_invariant.
+        intro_invariant votes_correct_invariant.
+        break_or_hyp; eauto.
+    - eauto.
+  Qed.
+
+  Lemma one_leaderLog_per_term_do_leader :
+    refined_raft_net_invariant_do_leader one_leaderLog_per_term.
+  Proof.
+    admit.
+  Qed.
+
+  Lemma one_leaderLog_per_term_do_generic_server :
+    refined_raft_net_invariant_do_generic_server one_leaderLog_per_term.
+  Proof.
+    admit.
+  Qed.
+
+  Lemma one_leaderLog_per_term_state_same_packet_subset :
+    refined_raft_net_invariant_state_same_packet_subset one_leaderLog_per_term.
+  Proof.
+    admit.
+  Qed.
+
+  Lemma one_leaderLog_per_term_reboot :
+    refined_raft_net_invariant_reboot one_leaderLog_per_term.
+  Proof.
+    admit.
+  Qed.
+
+  Lemma one_leaderLog_per_term_invariant :
     forall net,
       refined_raft_intermediate_reachable net ->
       one_leaderLog_per_term net.
-  Admitted.
+  Proof.
+    intros.
+    apply refined_raft_net_invariant; auto.
+    - apply one_leaderLog_per_term_init.
+    - apply one_leaderLog_per_term_client_request.
+    - apply one_leaderLog_per_term_timeout.
+    - apply one_leaderLog_per_term_append_entries.
+    - apply one_leaderLog_per_term_append_entries_reply.
+    - apply one_leaderLog_per_term_request_vote.
+    - apply one_leaderLog_per_term_request_vote_reply.
+    - apply one_leaderLog_per_term_do_leader.
+    - apply one_leaderLog_per_term_do_generic_server.
+    - apply one_leaderLog_per_term_state_same_packet_subset.
+    - apply one_leaderLog_per_term_reboot.
+  Qed.
 
   Instance ollpti : one_leaderLog_per_term_interface.
   Proof.
-    split. eauto using one_leaderLog_per_term_invariant.
+    split; intros; intro_invariant one_leaderLog_per_term_invariant;
+      red; eapply_prop one_leaderLog_per_term.
   Qed.
 
 End OneLeaderLogPerTerm.
