raft/OneLeaderLogPerTermInterface.v
@@ -17,12 +17,34 @@ Section OneLeaderLogPerTerm.
     forall h h' t ll ll',
       In (t, ll) (leaderLogs (fst (nwState net h))) ->
       In (t, ll') (leaderLogs (fst (nwState net h'))) ->
+      h = h' /\ ll = ll'.
+
+  (* convenience *)
+  Definition one_leaderLog_per_term_log (net : network) : Prop :=
+    forall h h' t ll ll',
+      In (t, ll) (leaderLogs (fst (nwState net h))) ->
+      In (t, ll') (leaderLogs (fst (nwState net h'))) ->
       ll = ll'.
+
+  (* convenience *)
+  Definition one_leaderLog_per_term_host (net : network) : Prop :=
+    forall h h' t ll ll',
+      In (t, ll) (leaderLogs (fst (nwState net h))) ->
+      In (t, ll') (leaderLogs (fst (nwState net h'))) ->
+      h = h'.
 
 
   Class one_leaderLog_per_term_interface : Prop :=
     {
       one_leaderLog_per_term_invariant :
+        forall net,
+          refined_raft_intermediate_reachable net ->
+          one_leaderLog_per_term net;
+      one_leaderLog_per_term_log_invariant :
+        forall net,
+          refined_raft_intermediate_reachable net ->
+          one_leaderLog_per_term_log net;
+      one_leaderLog_per_term_host_invariant :
         forall net,
           refined_raft_intermediate_reachable net ->
           one_leaderLog_per_term net
